PikeEquiv.v
@@ -1,0 +1,76 @@
+(* Relating the PikeVM smallstep semantics to the Pike Tree smallstep semantics *)
+
+Require Import List Lia.
+Import ListNotations.
+
+Require Import Regex Chars Groups.
+Require Import Tree Semantics BooleanSemantics.
+Require Import NFA PikeTree PikeVM.
+
+(* a tree and a thread are equivalent when they are about to execute the same thing *)
+(* this means when the tree represents a given regex and continuation, *)
+(* the thread is at a pc that will execute the nfa of that same regex and continuation *)
+Inductive tree_thread (code:code) (inp:input): (tree * group_map) -> LoopBool -> thread -> Prop :=
+| tt_eq:
+  forall tree gm pc b pc_cont pc_end r cont
+    (TREE: bool_tree r cont inp b tree)
+    (NFA: nfa_rep r code pc pc_cont)
+    (CONT: continuation_rep cont code pc_cont pc_end),
+    tree_thread code inp (tree, gm) b (pc, gm, b).
+
+(* the initial active thread and the initial active tree are related with the invariant *)
+Lemma initial_tree_thread:
+  forall r code tree inp
+    (COMPILE: compilation r = code)
+    (TREE: bool_tree r [] inp CanExit tree),
+    tree_thread code inp (tree, empty_group_map) CanExit (0, empty_group_map, CanExit).
+Proof.
+  intros r code tree inp COMPILE TREE.
+  unfold compilation in COMPILE. destruct (compile r 0) as [c fresh] eqn:COMP.
+  apply compile_nfa_rep with (prev := []) in COMP as REP; auto. simpl in REP.
+  apply fresh_correct in COMP. simpl in COMP. subst.
+  subst. eapply tt_eq with (pc_cont := length c) (pc_end := length c); eauto.
+  - simpl in REP. apply nfa_rep_extend. auto.
+  - constructor. replace (length c) with (length c + 0) by auto. rewrite get_prefix. auto.
+Qed.
+
+(* lifting the equivalence predicate to lists *)
+Inductive list_tree_thread (code:code) (inp:input) : list (tree * group_map) -> list thread -> Prop :=
+| ltt_nil: list_tree_thread code inp [] []
+| ltt_cons:
+  forall treelist threadlist tree gm pc b
+    (LTT: list_tree_thread code inp treelist threadlist)
+    (TT: tree_thread code inp (tree, gm) b (pc, gm, b)),
+    list_tree_thread code inp ((tree,gm)::treelist) ((pc,gm,b)::threadlist).
+
+(* relating the best matches *)
+Inductive best_eq (inp:input) : option leaf -> option thread -> Prop :=
+| best_none: best_eq inp None None
+| best_some:
+  forall gm pc b, best_eq inp (Some (inp, gm)) (Some (pc, gm, b)).
+
+(* lifting the equivalence predicate to pike states *)
+Inductive pike_inv (code:code): pike_tree_state -> pike_vm_state -> Prop :=
+| pikeinv:
+  forall inp idx treeactive treebest treeblocked threadactive threadbest threadblocked
+    (ACTIVE: list_tree_thread code inp treeactive threadactive)
+    (BEST: best_eq inp treebest threadbest)
+    (BLOCKED: list_tree_thread code inp treeblocked threadblocked),
+    pike_inv code (PTS idx treeactive treebest treeblocked) (PVS inp idx threadactive threadbest threadblocked).
+
+(* the initial states of both smallstep semantics are related with the invariant *)
+Lemma initial_pike_inv:
+  forall r inp tree code
+    (TREE: bool_tree r [] inp CanExit tree)
+    (COMPILE: compilation r = code),
+    pike_inv code (pike_tree_initial_state tree) (pike_vm_initial_state inp).
+Proof.
+  intros r inp tree code TREE COMPILE.
+  unfold compilation in COMPILE. destruct (compile r 0) as [c fresh] eqn:COMP.
+  apply compile_nfa_rep with (prev := []) in COMP as REP; auto. simpl in REP.
+  apply fresh_correct in COMP. simpl in COMP. subst.
+  constructor; constructor; try constructor.
+  apply tt_eq with (pc_cont:=length c) (pc_end:=length c) (r:=r) (cont:=[]); auto.
+  - subst. apply nfa_rep_extend. auto.
+  - constructor. replace (length c) with (length c + 0) by auto. rewrite get_prefix. auto.
+Qed.
